jessie: refine makeCounter security proof with proper cUp object modeling
- Redefine checked_counter to use full cUp object (jobj) instead of just cUpIncr
- Add c_up_val definition for the capability-restricted object with only 'incr' method
- Add wp_obj_get1 lemma for single-property object field lookup
- Add wp_c_up_get_incr lemma for specifically getting incr from c_up_val
- Add c_up_low lemma proving low capability for c_up_val
- Update use_closure_low to include object field lookup step
- Update checked_counter_spec proof to inline closure logic and use c_up_low
- This properly models capability separation where attacker only receives cUp object
  with incr method, not direct access to counter or decr method

theories/jessie/make_counter.v
@@ -84,18 +84,20 @@ Qed.
 
 Definition checked_counter : expr :=
   let: "c" := make_counter () in
-  let: "cUpIncr" := obj_get "c" incr_key in
-  let: "use" := (λ: "cUpIncr",
+  let: "cUp" := jobj ["incr" := obj_get "c" incr_key] in
+  let: "use" := (λ: "cUp",
     rec: "use" <> :=
+      let: "cUpIncr" := obj_get "cUp" incr_key in
       let: "n" := "cUpIncr" () in
-      assert: (#0 < "n")) "cUpIncr" in
-  (* TODO: change this back to the object-shaped cUp export once the proof
-     goes through cleanly with object lookup in both places. *)
-  ("use", "cUpIncr").
+      assert: (#0 < "n")) "cUp" in
+  ("use", "cUp").
 
 Definition counter_val (count : loc) : val :=
   j_objectV2 "incr" (RecV "f" <> (count += #1))
              "decr" (RecV "f" <> (count -= #1)).
+
+Definition c_up_val (count : loc) : val :=
+  (#object_tag, ((incr_key, RecV "f" <> (count += #1)), ()))%V.
 
 Section proof.
   Context `{heapG Σ}.
@@ -103,6 +105,28 @@ Section proof.
 
   Definition counter_inv (count : loc) : iProp Σ :=
     (inv N (∃ z : Z, ⌜0 ≤ z⌝ ∗ count ↦ #z))%I.
+
+  Lemma wp_obj_get1 k v :
+    {{{ True }}}
+      obj_get (jobj [k := (of_val v)]) (j_string k)
+    {{{ RET v; True }}}.
+  Proof.
+    iIntros (Φ) "HΦ". rewrite /obj_get /obj_get_fields.
+    wp_lam. wp_lam.
+    wp_proj. wp_let.
+    wp_proj. wp_let.
+    wp_apply wp_assert. wp_op=>?; last done.
+    iSplit; first done.
+    iNext. wp_finish. wp_rec. wp_let.
+    wp_op=>[EQ|NEQ].
+    - exfalso. by discriminate EQ.
+    - etrans; [|eapply wp_if_false]. wp_finish.
+    wp_proj. wp_let.
+    wp_proj. wp_let.
+    wp_proj.
+    wp_op=>[EQ'|NEQ']; [etrans; [|eapply wp_if_true]; wp_finish|exfalso; apply NEQ'; reflexivity].
+    wp_proj. by iApply "HΦ".
+  Qed.
 
   Lemma wp_obj_get2_first k1 k2 v1 v2 :
     {{{ True }}}
@@ -133,6 +157,29 @@ Section proof.
   Proof.
     rewrite /counter_val /incr_key.
     apply (wp_obj_get2_first "incr" "decr").
+  Qed.
+
+  Lemma wp_c_up_get_incr (count : loc) :
+    {{{ True }}}
+      obj_get (c_up_val count) incr_key
+    {{{ RET (RecV "f" <> (count += #1)); True }}}.
+  Proof.
+    rewrite /c_up_val.
+    iIntros (Φ) "HΦ". rewrite /obj_get /obj_get_fields.
+    wp_lam. wp_lam.
+    wp_proj. wp_let.
+    wp_proj. wp_let.
+    wp_apply wp_assert. wp_op=>?; last done.
+    iSplit; first done.
+    iNext. wp_finish. wp_rec. wp_let.
+    wp_op=>[EQ|NEQ].
+    - exfalso. by discriminate EQ.
+    - etrans; [|eapply wp_if_false]. wp_finish.
+    wp_proj. wp_let.
+    wp_proj. wp_let.
+    wp_proj.
+    wp_op=>[EQ'|NEQ']; [etrans; [|eapply wp_if_true]; wp_finish|exfalso; apply NEQ'; reflexivity].
+    wp_proj. by iApply "HΦ".
   Qed.
 
   Lemma make_counter_spec :
@@ -214,15 +261,30 @@ Section proof.
     iApply "HΦ". by simpl_low.
   Qed.
 
+  Lemma c_up_low count :
+    heap_ctx ∗ counter_inv count ⊢ low (c_up_val count).
+  Proof.
+    iIntros "#H". rewrite /c_up_val /incr_key /j_string.
+    simpl_low. iNext. iSplit; first done.
+    iNext. iSplit; last done.
+    iNext. iSplit.
+    - iNext. iSplit; done.
+    - by iApply (incr_closure_low with "H").
+  Qed.
+
   Lemma use_closure_low count :
     heap_ctx ∗ counter_inv count ⊢
       low (RecV "use" <>
-        (let: "n" := (rec: "f" <> := count += #1) () in
+        (let: "cUpIncr" := obj_get (c_up_val count) incr_key in
+         let: "n" := "cUpIncr" () in
          assert: (#0 < "n"))).
   Proof.
     iIntros "#(Hh & Hinv)". rewrite low_rec.
     iAlways. iNext. iIntros (? Φ) "_ HΦ". simpl_subst.
     wp_apply (wp_forget_progress progress).
+    wp_apply (wp_c_up_get_incr count).
+    iIntros "_".
+    wp_let.
     wp_apply (incr_call_pos with "[$Hh $Hinv]").
     iIntros (v) "Hv".
     iDestruct "Hv" as (z) "Hv".
@@ -252,8 +314,24 @@ Section proof.
     clear Φ.
     rewrite low_val /=. iNext.
     iSplitL.
-    - by iApply (use_closure_low with "[$Hh $Hinv]").
-    - by iApply (incr_closure_low with "[$Hh $Hinv]").
+    - rewrite low_rec.
+      iAlways. iNext. iIntros (? Ψ) "_ HΨ". simpl_subst.
+      wp_apply (wp_forget_progress progress).
+      wp_apply (wp_c_up_get_incr count).
+      iIntros "_".
+      wp_let.
+      wp_apply (incr_call_pos with "[$Hh $Hinv]").
+      iIntros (v) "Hv".
+      iDestruct "Hv" as (z) "Hv".
+      iDestruct "Hv" as "[Hv Hpos]".
+      iDestruct "Hv" as %Hv.
+      iDestruct "Hpos" as %Hpos.
+      subst v.
+      wp_let.
+      wp_apply wp_assert. wp_op=>?; last by exfalso; lia.
+      iSplit; first done.
+      by iApply "HΨ"; simpl_low.
+    - by iApply (c_up_low with "[$Hh $Hinv]").
   Qed.
 End proof.
 
